git/cruhland/lean4-axiomatic/Lean4Axiomatic/Natural/Impl/Nat.lean
@@ -1,74 +1,82 @@
-import Lean4Axiomatic.Eqv
 import Lean4Axiomatic.Natural
 import Lean4Axiomatic.Natural.Impl.Default
 import Lean4Axiomatic.Natural.Impl.Derived
 
 namespace Lean4Axiomatic.Natural.Impl.Nat
 
-open Relation (EqvOp?)
-
-instance constructors : Constructors Nat where
+instance constructors : Constructors Nat := {
   zero := Nat.zero
   step := Nat.succ
+}
 
-instance eqvOp? : EqvOp? Nat where
+instance eqvOp? : Relation.Equivalence.EqvOp? Nat := {
   tildeDash := Eq
   refl := λ {x} => Eq.refl x
   symm := Eq.symm
   trans := Eq.trans
   tildeDashQuestion := Nat.decEq
+}
 
-instance equality : Equality Nat where
+instance equality : Equality Nat := {
   eqvOp? := eqvOp?
+}
 
-instance literals : Literals Nat where
+instance literals : Literals Nat := {
   literal := @instOfNatNat
-  literal_zero := Eqv.refl
-  literal_step := Eqv.refl
+  literal_zero := Rel.refl
+  literal_step := Rel.refl
+}
 
 instance step_substitutive
-    : AA.Substitutive₁ (step : Nat → Nat) (· ≃ ·) (· ≃ ·) where
+    : AA.Substitutive₁ (step : Nat → Nat) (· ≃ ·) (· ≃ ·)
+    := {
   subst₁ := congrArg step
+}
 
-instance core : Core Nat where
+instance core : Core Nat := {
   step_substitutive := step_substitutive
+}
 
 theorem succ_injective {n m : Nat} : Nat.succ n = Nat.succ m → n = m
 | Eq.refl _ => Eq.refl _
 
-instance step_injective : AA.Injective (step : Nat → Nat) (· ≃ ·) (· ≃ ·) where
+instance step_injective : AA.Injective (step : Nat → Nat) (· ≃ ·) (· ≃ ·) := {
   inject := succ_injective
+}
 
 def ind
     {motive : Nat → Sort v}
-    (mz : motive 0) (ms : {n : Nat} → motive n → motive (Nat.succ n)) (n : Nat)
-    : motive n :=
-  match n with
-  | Nat.zero => mz
-  | Nat.succ n => ms (ind mz ms n)
+    (mz : motive 0) (ms : {n : Nat} → motive n → motive (Nat.succ n))
+    : (n : Nat) → motive n
+| Nat.zero => mz
+| Nat.succ n => ms (ind mz ms n)
 
-instance axioms_base : Axioms.Base Nat where
+instance axioms_base : Axioms.Base Nat := {
   step_injective := step_injective
   step_neq_zero := Nat.noConfusion
   -- 2022-01-11: Using `Nat.rec` directly here, gives the following error:
   -- code generator does not support recursor 'Nat.rec' yet, consider using
   -- 'match ... with' and/or structural recursion
   ind := ind
+}
 
-instance addition_base : Addition.Base Nat where
+instance addition_base : Addition.Base Nat := {
   addOp := _root_.instAddNat
   zero_add := @Nat.zero_add
   step_add := @Nat.succ_add
+}
 
-instance multiplication_base : Multiplication.Base Nat where
+instance multiplication_base : Multiplication.Base Nat := {
   mulOp := _root_.instMulNat
   zero_mul := @Nat.zero_mul
   step_mul := @Nat.succ_mul
+}
 
-instance exponentiation_base : Exponentiation.Base Nat where
+instance exponentiation_base : Exponentiation.Base Nat := {
   powOp := _root_.instPowNatNat
-  pow_zero {n : Nat} : n ^ 0 ≃ 1 := rfl
-  pow_step {n m : Nat} : n ^ step m ≃ n ^ m * n := rfl
+  pow_zero := rfl
+  pow_step := rfl
+}
 
 instance : Natural Nat where
   toCore := core
