git/cruhland/lean4-axiomatic/Lean4Axiomatic/Function.lean
@@ -1,0 +1,65 @@
+
+namespace Lean4Axiomatic
+namespace Function
+
+/-! # Definitions and properties pertaining to functions -/
+
+/--
+This class generalizes the symmetric and commutative properties.
+
+There are some useful results that apply both to symmetric and commutative
+operations. Using this class allows the results to be given by a single
+definition. See `Lean4Axiomatic.AA.substR_from_substL_swap` for an example.
+
+See `Swappable.swap` for details about the actual property.
+
+**Named parameters**
+- `α`: the argument type of the swappable binary operation `f`.
+- `β`: the result type of the swappable binary operation `f`.
+- `f`: the binary operation whose arguments are "swappable" under `R`.
+- `R`: the binary relation that holds between "swapped" invocations of `f`.
+-/
+class Swappable {α : Sort u} {β : Sort v} (f : α → α → β) (R : β → β → Prop) :=
+  /--
+  The relation `R` holds between any two invocations of `f` that have the same
+  arguments, but provided in the opposite order as each other.
+
+  There are many useful things that obey this property. If `β` is `Prop` and
+  `R` is implication (`· → ·`) then `f` is a symmetric relation. If `R` is
+  equality or an equivalence relation, then `f` is a commutative function.
+
+  **Named parameters**
+  - `x`, `y`: the arguments to `f`.
+  -/
+  swap : {x y : α} → R (f x y) (f y x)
+
+export Swappable (swap)
+
+/--
+If a relation `R` is swappable over one direction of an implication, then it is
+automatically swappable over the other direction (and therefore both).
+
+**Intuition**: If `R x y → R y x` for all `x` and `y`, then it must also be
+true that `R y x → R x y`, by substituting `y` for `x` and vice versa.
+
+**Named parameters**
+- `α`: the type of `R`'s arguments.
+- `R`: the swappable binary relation.
+
+**Class parameters**
+- `Swappable R (· → ·)`: evidence that `R` is swappable over implication.
+-/
+instance swappable_over_iff_from_swappable_over_implication
+    {α : Sort u} {R : α → α → Prop}
+    [inst : Swappable R (· → ·)] : Swappable R (· ↔ ·)
+    := {
+  swap := Iff.intro (swap (self := inst)) (swap (self := inst))
+}
+
+end Function
+
+namespace Fn
+export Function (swap Swappable)
+end Fn
+
+end Lean4Axiomatic
