git/cruhland/lean4-axiomatic/Lean4Axiomatic/Hand.lean
@@ -1,0 +1,29 @@
+
+namespace Lean4Axiomatic
+
+/-! # Handedness -/
+
+/--
+Handedness: either left-handed or right-handed.
+
+Intended to be used as a more meaniningful `Bool` type in contexts where it
+applies. One example is in selecting the left- or right-hand side of an ordered
+pair. Another is in specifying which side of a binary operator an algebraic
+property acts on; a common one is the concept of a left inverse (`a⁻¹ * a ≃ 1`)
+vs. a right inverse (`a * a⁻¹ ≃ 1`).
+-/
+inductive Hand where
+| /-- Left hand.  -/ L
+| /-- Right hand. -/ R
+
+/--
+Selects the left-hand or right-hand argument, according to the given `Hand`.
+
+**Named parameters**
+- `α`: The `Sort` of the items to select.
+-/
+abbrev Hand.pick {α : Sort u} : Hand → α → α → α
+| L, x, y => x
+| R, x, y => y
+
+end Lean4Axiomatic
