git/cruhland/lean4-axiomatic/Lean4Axiomatic/Relation/Equivalence.lean
@@ -1,0 +1,2 @@
+import Lean4Axiomatic.Relation.Equivalence.Core
+import Lean4Axiomatic.Relation.Equivalence.Impl
