git/cruhland/lean4-axiomatic/Lean4Axiomatic/Relation/Equivalence/Core.lean
@@ -1,0 +1,267 @@
+import Lean4Axiomatic.Function
+import Lean4Axiomatic.Operators
+
+/-!
+# Equivalence relations
+
+## Fundamental definitions and properties
+-/
+
+namespace Lean4Axiomatic
+namespace Relation
+
+/--
+Class for
+[reflexive relations](https://en.wikipedia.org/wiki/Reflexive_relation).
+
+Paraphrasing Wikipedia, a homogeneous binary relation `R` on a sort `α` is
+**reflexive** iff it relates every inhabitant of `α` to itself.
+
+This property is provided by the single field `Reflexive.refl`; see its
+documentation for more details.
+
+**Named parameters**
+- `α`: The `Sort` of `R`'s parameters.
+- `R`: The homogeneous binary relation obeying the reflexive property.
+-/
+class Reflexive {α : Sort u} (R : α → α → Prop) :=
+  /--
+  The reflexive property of a homogeneous binary relation `R` on a sort `α`.
+
+  Equality, or equivalence, are the archetypes of reflexive relations: if a
+  sort `α` has an equivalence relation (see `Eqv` and `EqvOp`), then any
+  inhabitant `x : α` is equivalent to itself (i.e., `x ≃ x`).
+
+  Another reflexive relation is _divisibility_, from number theory. We say an
+  integer `a` divides an integer `b` iff `b ≃ c * a` for some integer `c`. We
+  can show that all integers divide themselves by taking `c ≃ 1`.
+
+  An example of a relation that is _not_ reflexive is "`n * m` is even" for
+  natural numbers `n`, `m`. While "`n * n` is even" holds for even numbers `n`,
+  it fails for odd numbers and thus is not reflexive on the natural numbers.
+  Credit goes to Wikipedia for this example.
+
+  **Named parameters**
+  - See `Reflexive` for the parameters provided by the class.
+  - `x`: `R`'s first and second argument.
+  -/
+  refl : {x : α} → R x x
+
+export Reflexive (refl)
+
+/--
+The type of logical implication (i.e., the arrow type or exponential) is
+reflexive: there are inhabitants of the type `α → α` for all `α : Prop`.
+
+**Intuition**: The identity function (i.e, the function that simply returns its
+single argument) meets this requirement.
+-/
+instance implication_reflexive : Reflexive (· → ·) := {
+  refl := id
+}
+
+/--
+Class for
+[symmetric relations](https://en.wikipedia.org/wiki/Symmetric_relation).
+
+A homogeneous binary relation `R` on a sort `α` is **symmetric** iff its truth
+value remains the same when its arguments are exchanged.
+
+This property is provided by the single field `Symmetric.symm`; see its
+documentation for more details.
+
+**Named parameters**
+- `α`: The `Sort` of `R`'s parameters.
+- `R`: The homogeneous binary relation obeying the symmetric property.
+-/
+class Symmetric {α : Sort u} (R : α → α → Prop) :=
+  /--
+  The symmetric property of a homogeneous binary relation `R` on a sort `α`.
+
+  Equality, or equivalence, are the archetypes of symmetric relations: if a
+  sort `α` has an equivalence relation (see `Eqv` and `EqvOp`), and for some
+  inhabitants `x y : α` we know that `x` is equivalent to `y` (i.e., `x ≃ y`),
+  then we also know that `y` is equivalent to `x` (i.e., `y ≃ x`).
+
+  Another example is actually the non-example from `Reflexive.refl`,
+  "`n * m` is even" for natural numbers `n` and `m`. In this case it's because
+  multiplication of natural numbers is commutative.
+
+  A relation that fails to be symmetric is "X likes Y" where X and Y are
+  people. While there are many specific Xs and Ys that like each other, this
+  unfortunately doesn't hold in general.
+
+  **Named parameters**
+  - See `Symmetric` for the parameters provided by the class.
+  - `x`, `y`: The arguments to `R`.
+  -/
+  symm : {x y : α} → R x y → R y x
+
+export Symmetric (symm)
+
+/--
+`Symmetric` relations are special cases of `Fn.Swappable` functions.
+
+**Intuition**: Just going by syntax, a relation `R` that satisfies
+`Symmetric.symm` also satisfies `Fn.swap` as the swappable function `f`, with
+logical implication (i.e., the function type or arrow type) as the relation
+between swapped invocations.
+
+**Named parameters**
+- `α`: The `Sort` of `R`'s parameters.
+- `R`: The symmetric relation.
+
+**Class parameters**
+- `Symmetric R`: Evidence that `R` is symmetric.
+-/
+instance swappable_over_implication_from_symmetric
+    {α : Sort u} {R : α → α → Prop} [Symmetric R] : Fn.Swappable R (· → ·)
+    := {
+  swap := symm
+}
+
+/--
+The negation of a symmetric relation is also symmetric.
+
+**Intuition**: Consider the set of all input pairs to the relation. It can be
+divided into two disjoint subsets: the pairs that satisfy the relation, and
+the pairs that don't. Both subsets must be closed under the operation of
+swapping the components of the pairs, otherwise the relation wouldn't be
+symmetric.
+
+**Named parameters**
+- `α`: The `Sort` of `R`'s parameters.
+- `R`: The symmetric relation.
+
+**Class parameters**
+- `Symmetric R`: Evidence that `R` is symmetric.
+-/
+instance negation_preserves_symmetry
+    {α : Sort u} {R : α → α → Prop} [Symmetric R] : Symmetric (¬ R · ·)
+    := {
+  symm := mt symm
+}
+
+/--
+Class for
+[transitive relations](https://en.wikipedia.org/wiki/Transitive_relation).
+
+A homogeneous binary relation `R` on a sort `α` is **transitive** iff when `R`
+relates `x` to `y`, and `y` to `z`, then it also relates `x` to `z`, for all
+`x`, `y`, and `z` inhabiting `α`. Transitive relations are useful because new
+pairs of values can be shown to be related by chaining already known pairs
+together.
+
+This property is provided by the single field `Transitive.trans`; see its
+documentation for more details.
+
+**Named parameters**
+- `α`: The `Sort` of `R`'s parameters.
+- `R`: The homogeneous binary relation obeying the transitive property.
+-/
+class Transitive {α : Sort u} (R : α → α → Prop) :=
+  /--
+  The transitive property of a homogeneous binary relation `R` on a sort `α`.
+
+  Equality, or equivalence, are the archetypes of transitive relations: if a
+  sort `α` has an equivalence relation (see `Eqv` and `EqvOp`), and for some
+  inhabitants `x y z : α` we know that `x` is equivalent to `y` (i.e. `x ≃ y`)
+  and `y` is equivalent to `z` (i.e. `y ≃ z`), then we also know that `x` is
+  equivalent to `z` (i.e. `x ≃ z`).
+
+  Another transitive relation is _divisibility_, from number theory. We say an
+  integer `a` divides an integer `b` iff `b ≃ c * a` for some integer `c`. If
+  we know that `x` divides `y` (into, say, `p` copies of `x`), and `y` divides
+  `z` (into `q` copies of `y`), then `z` must consist of `p * q` copies of `x`,
+  and therefore `x` divides `z`.
+
+  A relation that fails to be transitive is "X likes Y" where X and Y are
+  people. If Alice likes Bob, and Bob likes Carol, then Alice might be a bit
+  jealous of Carol, and definitely not inclined to like her!
+
+  **Named parameters**
+  - See `Transitive` for the parameters provided by the class.
+  - `x`, `y`, `z`: The arguments to `R`.
+  -/
+  trans : {x y z : α} → R x y → R y z → R x z
+
+export Transitive (trans)
+
+/--
+`Transitive` is a special case of the `Trans` class from Lean's Prelude.
+
+**Intuition**: The Prelude's `Trans` allows the three values involved in the
+property to be of different sorts. Which means it must support three
+heterogeneous relations to pair up the values. Our `Transitive` is the special
+case where all values are of the same sort, and only one homogeneous relation
+is needed.
+
+**Named parameters**
+- `α`: The `Sort` of `R`'s parameters.
+- `R`: The transitive relation.
+
+**Class parameters**
+- `Transitive R`: Evidence that `R` is transitive.
+-/
+instance prelude_trans_from_transitive
+    {α : Sort u} {R : α → α → Prop} [Transitive R] : Trans R R R
+    := {
+  trans := trans
+}
+
+/--
+Logical implication (i.e. the function type or the arrow type) is transitive.
+
+**Intuition**: This is essentially why implications are so useful in logic,
+because intermediate deductions can be combined into a larger, more significant
+result. Alternatively, this is just function composition.
+-/
+instance implication_transitive : Transitive (· → ·) := {
+  trans := flip Function.comp
+}
+
+namespace Equivalence
+
+/--
+Class for
+[equivalence relations](https://en.wikipedia.org/wiki/Equivalence_relation).
+
+A homogeneous binary relation `R` on a sort `α` is an **equivalence relation**
+iff it is reflexive, symmetric, and transitive.
+
+Equality is the simplest example of an equivalence relation, where each
+inhabitant of `α` is equivalent only to itself. A less trivial example is the
+relation where two integers are equivalent iff they have the same sign.
+
+**Named parameters**
+- `α`: The `Sort` of `R`'s parameters.
+- `R`: The equivalence relation.
+-/
+class Eqv {α : Sort u} (R : α → α → Prop)
+    extends Reflexive R, Symmetric R, Transitive R
+
+/--
+Provides an equivalence relation over `α` with the operator `· ≃ ·`.
+
+**Named parameters**
+- `α`: The `Sort` of the elements in the relation.
+-/
+class EqvOp (α : Sort u) extends Operators.TildeDash α, Eqv tildeDash
+
+/--
+Extends `EqvOp` with `· ≃? ·`, a decision procedure for equivalence.
+
+**Named parameters**
+- `α`: The `Sort` of the elements in the relation.
+-/
+class EqvOp? (α : Sort u)
+    extends EqvOp α, Operators.TildeDashQuestion tildeDash
+
+end Equivalence
+end Relation
+
+namespace Rel
+export Relation (refl symm trans)
+end Rel
+
+end Lean4Axiomatic
