git/cruhland/lean4-axiomatic/Lean4Axiomatic/Relation/Equivalence/Impl.lean
@@ -1,0 +1,253 @@
+import Lean4Axiomatic.Hand
+import Lean4Axiomatic.Operators
+import Lean4Axiomatic.Relation.Equivalence.Core
+
+namespace Lean4Axiomatic.Relation.Equivalence.Impl
+
+/-! # Implementations of equivalence relations -/
+
+namespace DepFn
+
+/-! ## For dependent functions -/
+
+variable {α : Sort u}
+variable {β : α → Sort v}
+variable (indexed_eqvOp : {x : α} → EqvOp (β x))
+
+/--
+The "pointwise" equivalence relation for dependent functions.
+
+Two dependent functions are considered to be equivalent if their outputs are
+equivalent for every inhabitant of their domain.
+
+**Named parameters**
+- `α`: The domain of the dependent functions.
+- `β`: The codomain family of the dependent functions.
+- `indexed_eqvOp`: Evidence that all codomains have an equivalence relation.
+- `f₁`, `f₂`: The dependent functions to evaluate for equivalence.
+-/
+def eqv (f₁ f₂ : (x : α) → β x) : Prop := ∀ (x : α), f₁ x ≃ f₂ x
+
+/--
+The reflexive property of pointwise equivalence for dependent functions.
+
+**Intuition**: We need to show that `f x ≃ f x` for every `x : α`. But this
+follows immediately (by `refl`) from the `EqvOp (β x)` instance obtained from
+`indexed_eqvOp` for each `x`.
+
+Note on syntax: the `· ≃ ·` operator could not be used in the type signature
+because the equivalence relation requires the `indexed_eqvOp` argument in
+addition to its typical arguments.
+
+**Named parameters**
+- `α`: The domain of the dependent functions.
+- `β`: The codomain family of the dependent functions.
+- `indexed_eqvOp`: Evidence that all codomains have an equivalence relation.
+- `f`: The function to evaluate for equivalence to itself.
+-/
+theorem refl
+    {f : (x : α) → β x}
+    : eqv indexed_eqvOp f f
+    := by
+  show ∀ (x : α), f x ≃ f x
+  intro x
+  exact indexed_eqvOp.refl
+
+/--
+The symmetric property of pointwise equivalence for dependent functions.
+
+**Intuition**: We need to show that `f x ≃ g x → g x ≃ f x` for every `x : α`.
+But this follows immediately (by `symm`) from the `EqvOp (β x)` instance
+obtained from `indexed_eqvOp` for each `x`.
+
+Note on syntax: the `· ≃ ·` operator could not be used in the type signature
+because the equivalence relation requires the `indexed_eqvOp` argument in
+addition to its typical arguments.
+
+**Named parameters**
+- `α`: The domain of the dependent functions.
+- `β`: The codomain family of the dependent functions.
+- `indexed_eqvOp`: Evidence that all codomains have an equivalence relation.
+- `f`, `g`: The dependent functions that are arguments to the relation.
+-/
+theorem symm
+    {f g : (x : α) → β x}
+    : eqv indexed_eqvOp f g → eqv indexed_eqvOp g f
+    := by
+  intro (_ : ∀ (x : α), f x ≃ g x)
+  show ∀ (x : α), g x ≃ f x
+  intro x
+  have : f x ≃ g x := ‹∀ (x : α), f x ≃ g x› x
+  exact indexed_eqvOp.symm ‹f x ≃ g x›
+
+/--
+The transitive property of pointwise equivalence for dependent functions.
+
+**Intuition**: We need to show that `f x ≃ g x → g x ≃ h x → f x ≃ h x` for
+every `x : α`. But this follows immediately (by `trans`) from the `EqvOp (β x)`
+instance obtained from `indexed_eqvOp` for each `x`.
+
+Note on syntax: the `· ≃ ·` operator could not be used in the type signature
+because the equivalence relation requires the `indexed_eqvOp` argument in
+addition to its typical arguments.
+
+**Named parameters**
+- `α`: The domain of the dependent functions.
+- `β`: The codomain family of the dependent functions.
+- `indexed_eqvOp`: Evidence that all codomains have an equivalence relation.
+- `f`, `g`, `h`: The dependent functions that are arguments to the relation.
+-/
+theorem trans
+    {f g h : (x : α) → β x}
+    : eqv indexed_eqvOp f g → eqv indexed_eqvOp g h → eqv indexed_eqvOp f h
+    := by
+  intro (_ : ∀ (x : α), f x ≃ g x) (_ : ∀ (x : α), g x ≃ h x)
+  show ∀ (x : α), f x ≃ h x
+  intro x
+  have : f x ≃ g x := ‹∀ (x : α), f x ≃ g x› x
+  have : g x ≃ h x := ‹∀ (x : α), g x ≃ h x› x
+  exact indexed_eqvOp.trans ‹f x ≃ g x› ‹g x ≃ h x›
+
+/--
+Generates a "pointwise" equivalence relation (with its essential properties)
+for dependent functions, from evidence that every codomain in the functions'
+indexed family of output `Sort`s has an equivalence relation.
+
+More intuitively, a dependent function can be viewed as a generalization of a
+tuple. Each inhabitant `x : α` of the function's domain is an index to a unique
+tuple element. Just as in an ordinary tuple, the `Sort` of each element can be
+different; here it is given by `β x`. Comparing tuples for equivalence requires
+that each element be comparable in turn: the first elements must be equivalent,
+and the second elements, and the third, etc. This is what is meant by the term
+"pointwise". The `indexed_eqvOp` parameter provides the necessary equivalence
+relations for every tuple element.
+
+Thus, due to the `indexed_eqvOp` parameter, this definition is not directly
+useful as an `instance` of `EqvOp`. Instead, every caller of this function is
+expected to declare the result as an instance, specific to a particular use
+case.
+
+**Named parameters**
+- `α`: The domain of the dependent functions.
+- `β`: The codomain family of the dependent functions.
+- `indexed_eqvOp`: Evidence that all codomains have an equivalence relation.
+-/
+def eqvOp : EqvOp ((x : α) → β x) := {
+  tildeDash := eqv indexed_eqvOp
+  refl := refl indexed_eqvOp
+  symm := symm indexed_eqvOp
+  trans := trans indexed_eqvOp
+}
+
+end DepFn
+
+namespace Mapped
+
+/-! ## For types that convert into types having equivalence -/
+
+/--
+Extends an equivalence relation via a mapping between types.
+
+More concretely, given a sort `β` that has an equivalence relation, and a
+function `f` from a sort `α` into `β`, this definition generates an equivalence
+relation for `α`. It can save quite a lot of effort if writing the mapping
+between `α` and `β` is simple.
+
+Since the behavior of the equivalence relation depends completely upon the
+explicit parameter `f`, this definition is not directly useful as an `instance`
+of `EqvOp`. Instead, every caller of this function is expected to declare the
+result as an instance, specific to a particular use case.
+
+**Named parameters**
+- `α`: The `Sort` to generate an equivalence relation for.
+- `β`: The `Sort` that already has an equivalence relation.
+- `f`: The mapping from `α` to `β`.
+
+**Class parameters**
+- `EqvOp β`: The equivalence relation on `β`.
+-/
+def eqvOp
+    {α : Sort u} {β : Sort v} (f : α → β) [β_eqvOp : EqvOp β] : EqvOp α
+    := {
+  tildeDash := λ x y => f x ≃ f y
+  refl := β_eqvOp.refl
+  symm := β_eqvOp.symm
+  trans := β_eqvOp.trans
+}
+
+end Mapped
+
+namespace Prod
+
+/-! ## For product types (i.e. ordered pairs) -/
+
+variable {α β : Type}
+variable [EqvOp α]
+variable [EqvOp β]
+
+/--
+Converts an ordered pair into its dependent function representation.
+
+This function is a supporting definition for `Prod.eqvOp`, and is likely not
+very useful on its own.
+
+**Intuition**: The `Hand` parameter of the dependent function selects the
+associated component of the ordered pair to return. Since there are exactly two
+values of `Hand`, there are exactly two result types of the dependent
+function, and thus it fully reproduces the state of the pair.
+
+**Named parameters**
+- `α`: The `Type` of the pair's left element.
+- `β`: The `Type` of the pair's right element.
+-/
+def depFn_from_prod : α × β → ((hand : Hand) → hand.pick α β)
+| (a, b), Hand.L => a
+| (a, b), Hand.R => b
+
+/--
+Evidence that all codomains in the dependent function representation of ordered
+pairs have equivalence relations.
+
+This function is a supporting definition for `Prod.eqvOp`, and is likely not
+very useful on its own.
+
+**Intuition**: As the `indexed_eqvOp` argument to `DepFn.eqvOp`, this function
+provides evidence that there is an equivalence relation for every component of
+an ordered pair. Since there are only two components, this can easily be done
+by explicitly listing all associations.
+
+**Named parameters**
+- `α`: The `Type` of the codomain for `Hand.L`.
+- `β`: The `Type` of the codomain for `Hand.R`.
+
+**Class parameters**
+- `EqvOp α`: Evidence that `α` has an equivalence relation.
+- `EqvOp β`: Evidence that `β` has an equivalence relation.
+-/
+def indexed_eqvOp : {hand : Hand} → EqvOp (hand.pick α β)
+| Hand.L => ‹EqvOp α›
+| Hand.R => ‹EqvOp β›
+
+/--
+The standard ("pointwise") equivalence relation on ordered pairs whose left-
+and right-handed component types both have their own equivalence relations.
+
+**Implementation intuition**: Uses `Prod.indexed_eqvOp` and
+`Prod.depFn_from_prod` to produce an equivalence relation on the dependent
+function representation of ordered pairs, and extend it back to the original
+type `α × β`.
+
+**Named parameters**
+- `α`: The left-hand component type.
+- `β`: The right-hand component type.
+
+**Class parameters**
+- `EqvOp α`: Evidence that `α` has an equivalence relation.
+- `EqvOp β`: Evidence that `β` has an equivalence relation.
+-/
+instance eqvOp : EqvOp (α × β) :=
+  Mapped.eqvOp depFn_from_prod (β_eqvOp := DepFn.eqvOp indexed_eqvOp)
+
+end Prod
+
+end Lean4Axiomatic.Relation.Equivalence.Impl
